\begin{enumerate}[\bfseries \mbox{Ejercicio} 1.]

    %---------- Ejercicio 1 ----------
    \item \textbf{Demuestre que \boldmath $\Proy_{\vec{c}}=\Proy_{\vec{c}}\vec{a}+\Proy_{\vec{c}}\vec{b}$.\\\\
	Demostraci贸n.-}\; Sean $\vec{a},\vec{b},\vec{c}\in V_n$. Por definici贸n se tiene,
	$$\begin{array}{rcl}
	    \Proy_{\vec{c}}(\vec{a}+\vec{b})&=&\dfrac{(\vec{a}+\vec{b}\circ \vec{c}}{\|\vec{c}\|^2}\cdot \vec{c}\\\\
					    &=&\dfrac{\vec{a}\circ \vec{c}+\vec{b}\circ \vec{c}}{\|\vec{c}\|^2}\cdot \vec{c}\\\\
					    &=&\left(\dfrac{\vec{a}\circ \vec{c}}{\|\vec{c}\|^2}+\dfrac{\vec{b}\circ \vec{c}}{\|\vec{c}\|^2}\right)\cdot \vec{c}\\\\
					    &=&\dfrac{\vec{a}\circ \vec{c}}{\|\vec{c}\|^2}\cdot \vec{c}+\dfrac{\vec{b}\circ \vec{c}}{\|\vec{c}\|^2}\cdot \vec{c}\\\\
			   &=&\Proy_{\vec{c}} \vec{a}+\Proy_{\vec{c}} \vec{b}.\\\\
	\end{array}$$
	\vspace{.6cm}

    %---------- Ejercicio 2 ----------
    \item \textbf{\boldmath Si $\vec{b} \parallel \vec{c} \neq \vec{0}$. Muestre que $\Proy_{\vec{b}} \vec{a} = \Proy_{\vec{b}} \vec{a}$.\\\\
	Demostraci贸n.-}\; Sean $\vec{a},\vec{b},\vec{c}\in V_n$. Por definici贸n y dado que $\vec{b}=r\vec{c}$ para $r\in V\;r\neq 0$ se tiene,
	$$\begin{array}{rcl}
	    \Proy_{\vec{b}} \vec{a} &=& \dfrac{\vec{a}\circ \vec{b}}{\|\vec{b}\|^2}\cdot \vec{b}\\\\
				    &=&\dfrac{\vec{a}\circ (r\vec{c})}{\|r\vec{c}\|^2}\cdot (r\vec{c})\\\\
				    &=&\dfrac{r^2(\vec{a}\circ \vec{c})}{|r^2|\|\vec{c}\|^2}\cdot \vec{c}\\\\
				    &=&\dfrac{\vec{a}\circ \vec{c}}{\|\vec{c}\|^2}\cdot \vec{c}\\\\
				    &=&\Proy_{\vec{c}}\vec{a}.\\\\
	\end{array}$$


\end{enumerate}
